{
 "cells": [
  {
   "cell_type": "markdown",
   "metadata": {},
   "source": [
    "# Project 1.3\n",
    "### Conside the Cauchy problem\n",
    "$$\n",
    "u'(t) = -u(t)\\\\\n",
    "u(0) = 1'\n",
    "$$\n",
    "which we know has the analytical solution $u(t) = e^{-t}$.\n",
    "## (a) Show that the numerical solution computed by the forward Euler method is given by\n",
    "$$\n",
    "v_{m} = (1-\\Delta t)^m\\qquad m = 0,1,...\n",
    "$$\n",
    "## The forward Euler formula is given by\n",
    "$$\n",
    "\\frac{v_{m+1} - v_{m}}{\\Delta t} = -v_{m}\\\\\n",
    "v_{m+1} = v_{m} - v_{m}\\Delta t\\\\\n",
    "v_{m+1} = (1- \\Delta t)v_{m}\n",
    "$$\n",
    "# Using the initial condition yields\n",
    "$$\n",
    "v_{1} = 1- \\Delta t. \n",
    "$$\n",
    "## Based on this, assume that\n",
    "$$ \n",
    "v_{m} = (1-\\Delta t)^m,\\qquad m = 0,1,..\n",
    "$$\n",
    "## and show that this holds for $v_{m+1}$.\n",
    "$$\n",
    "v_{m+1} = (1-\\Delta t)v_{m}\\\\\n",
    "v_{m+1} = (1-\\Delta t)(1-\\Delta t)^m\\\\\n",
    "v_{m+1} = (1-\\Delta t)^{m+1}\\\\\n",
    "$$\n",
    "## (b) Show that $v_{m}$ converges toward the correct solution at $t = 1$ as $\\Delta t$ tends to zero.\n",
    "## Let the final time be $T = 1 = \\Delta tM$. This means that $\\Delta t= \\frac{1}{M}$, and $ \\lim_{M \\to \\infty} = \\lim_{ \\Delta t \\to 0}$.\n",
    "$$ \n",
    "v_{M} = (1 - \\frac{1}{M})^{M}\\\\\n",
    "$$\n",
    "## By the definition of the exponential\n",
    "$$\n",
    "\\lim_{M \\to \\infty} (1 - \\frac{1}{M})^{M} = e^{1}\n",
    "$$\n",
    "## (c) Show that \n",
    "$$\n",
    "\\frac{ u(t_{m+1}) - u(t_{m})}{ \\Delta t} \\approx u'(t_{m}) = f(u(t_{m}))\n",
    "$$\n",
    "## Derive the approximation to the derivative using the backwards difference  method and Taylor's theorem. The backwards difference scheme is\n",
    "$$\n",
    "\\frac{u(t_{m}) - u(t_{m} - \\Delta t)}{\\Delta t}\n",
    "$$\n",
    "## Evaluate the second term using a Taylor Expansion\n",
    "$$ \n",
    "u(t_{m} - \\Delta t) = u(t_{m}) + u'(t_{m})(- \\Delta t) + \\frac{u''(c)}{2}(\\Delta t)^2\\\\\n",
    "u'(t_{m}) = \\frac{u(t_{m}) - u(t_{m} - \\Delta t)}{\\Delta t} + O(\\Delta t) = f(u(t_{m}))\n",
    "$$ \n",
    "## which is equivalent to\n",
    "$$\n",
    "u'(t_{m+1}) = \\frac{u(t_{m+1}) - u(t_{m})}{\\Delta t} + O(\\Delta t) = f(u(t_{m+1})).\n",
    "$$\n",
    "## (d) Use this definition of the derivative to derive the backward Euler method.\n",
    "## Drop the error term, $O(\\Delta t)$ from the backward difference method,\n",
    "$$\n",
    "\\frac{v_{m+1} - v_{m}}{\\Delta t} = f(v_{m+1})\\\\\n",
    "v_{m+1} - \\Delta tf(v_{m+1}) = v_{m}\n",
    "$$\n",
    "## (e) Apply the backward Euler method to this Cauchy problem and show that \n",
    "$$\n",
    "v_{m} = \\frac{1}{(1+ \\Delta t)^m},\\qquad m = 0,1,...\n",
    "$$\n",
    "## Use induction to show this. First start with initial condition $u(0) = 1$ .\n",
    "$$\n",
    "v_{1} - \\Delta t(-v_{1}) = 1\\\\\n",
    "v_{1}(1+\\Delta t) = 1\\\\\n",
    "v_{1} = \\frac{1}{1+\\Delta t}\n",
    "$$\n",
    "## Now assume the hypothesis for $v_{m}$, and prove for $v_{m+1}$.\n",
    "$$\n",
    "v_{m+1} + \\Delta tv_{m+1} =  v_{m}\\\\\n",
    "v_{m+1} + \\Delta tv_{m+1} =\\frac{1}{(1+\\Delta t)}^m\\\\\n",
    "v_{m+1}(1 +\\Delta t) = \\frac{1}{(1+\\Delta t)}^m\\\\\n",
    "v_{m+1} = \\frac{1}{(1+\\Delta t)}^{m+1}\n",
    "$$\n",
    "## QED\n",
    "\n",
    "## (f) (i) Explain why \n",
    "$$\n",
    "\\frac{ u(t_{m+1}) - u(t_{m})}{ \\Delta t} \\approx \\frac{1}{2}(f(u(t_{m+1}))+ f(u(t_{m})))\n",
    "$$\n",
    "## (ii) and use this to derive the scheme\n",
    "$$\n",
    "v_{m+1} - \\frac{1}{2} \\Delta t f(v_{m+1}) = v_{m} +\\frac{1}{2} \\Delta tf(v_{m})\n",
    "$$\n",
    "## (i)The above equation could be derived using the central difference method, and establishing another time point in between $t_{m+1}$ and $t_{m}$. The above form would just be the average value of the function between these two time points. \n",
    "## (ii) Derive the above scheme by dropping the approximation sign, AKA the error term\n",
    "$$\n",
    "\\frac{(v_{m+1} - v_{m})}{ \\Delta t} = \\frac{1}{2}(f(v_{m+1})+ f(v_{m}))\\\\\n",
    "v_{m+1} - v_{m} = \\frac{1}{2}\\Delta t(f(v_{m+1}) + f(v_{m}))\\\\\n",
    "v_{m+1} - \\frac{1}{2}\\Delta tf(v_{m+1}) = \\frac{1}{2}\\Delta tf(v_{m}) + v_{m}\n",
    "$$\n",
    "## (g) Using the above scheme and the Cauchy problem show that\n",
    "$$\n",
    "v_{m} = (\\frac{2-\\Delta t}{2+\\Delta t})^m\n",
    "$$\n",
    "## Use induction to derive this. First use the initial condition to establish a base case.\n",
    "$$\n",
    "v_{1} + \\frac{1}{2} \\Delta t(v_{1}) = 1 - \\frac{1}{2}\\Delta t\\\\\n",
    "v_{1}(1+\\frac{1}{2}\\Delta t) = 1 - \\frac{1}{2} \\Delta t\\\\\n",
    "v_{1} = \\frac{1 - \\frac{1}{2 \\Delta t}}{1+\\frac{1}{2} \\Delta t}\\\\\n",
    "v_{1} = \\frac{2 - \\Delta t}{2 +\\Delta t}\n",
    "$$\n",
    "## Now assume the hypothesis for $v_{m}$ and prove for $v_{m+1}$.\n",
    "$$\n",
    "v_{m+1} + \\frac{1}{2}\\Delta tf(v_{m+1}) = -\\frac{1}{2}\\Delta tv_{m} + v_{m}\\\\\n",
    "v_{m+1} + \\frac{1}{2}\\Delta tf(v_{m+1} = -\\frac{1}{2}\\Delta t (\\frac{2-\\Delta t}{2+\\Delta t})^m +(\\frac{2-\\Delta t}{2+\\Delta t})^m\\\\\n",
    "v_{m+1}( 2 + \\Delta t) = (\\frac{2-\\Delta t}{2+\\Delta t})^m(2 - \\Delta t)\\\\\n",
    "v_{m+1} = (\\frac{2-\\Delta t}{2+\\Delta t})^m \\frac{(2 - \\Delta t)}{( 2 + \\Delta t)}\\\\\n",
    "v_{m+1} = (\\frac{2-\\Delta t}{2+\\Delta t})^{m+1}\n",
    "$$\n",
    "## QED\n",
    "\n",
    "\n",
    "\n",
    "\n"
   ]
  },
  {
   "cell_type": "markdown",
   "metadata": {},
   "source": [
    "## (h) Compare the accuracy of these three methods by computing approximations to the solutions of (1.65) at $ t=1$. Use the technique diplayed in Table 1.1 and project 1.1 to argue that the errors when using the schemes that have been derived in this project are $O(\\Delta t)$, $O(\\Delta t)$, and $O(\\Delta t^2)$ respectively.\n",
    "## I will do so using the same methods used in 1.1, in which we look at the rate of convergence $\\alpha$, which is given by the following formula.\n",
    "$$ \\large |z_n-z| \\leq c\\left(\\frac{1}{n}\\right)^\\alpha. $$\n",
    "## $\\alpha$ is solved for by taking the logarithm of this equation to yield a linear equation\n",
    "$$\\large \\ln |z_n-z| \\leq \\alpha \\ln (c/n) = \\alpha (\\ln c + \\ln (1/n)), $$\n",
    "## and then using polyfit in numpy to fit the slope $\\alpha$.\n",
    "## The following script does just that for the provided values of m, or dt, and demonstrated linear convergence for the forward and backward Euler method, and converges superlinearly for the central difference Euler method."
   ]
  },
  {
   "cell_type": "code",
   "execution_count": 28,
   "metadata": {
    "collapsed": false
   },
   "outputs": [
    {
     "name": "stdout",
     "output_type": "stream",
     "text": [
      "The convergence  rate of forward difference Euler method is: 1.00282054909\n",
      "The convergence  rate of backward difference Euler method is: 0.997317830809\n",
      "The convergence  rate of central difference Euler method is: 1.66186036994\n"
     ]
    }
   ],
   "source": [
    "import matplotlib as plt\n",
    "import numpy as np\n",
    "import math\n",
    "def fproj(m,type):\n",
    "    if type == 1:\n",
    "        x_new = (np.float(1)- np.float(1)/m)**m \n",
    "        x_dif = x_new - math.exp(-1)\n",
    "        x_lim1 = np.log(np.abs(x_dif))\n",
    "        line1_params = np.polyfit(np.log(1./m), x_lim1, 1)\n",
    "        return line1_params\n",
    "    elif type == 2:\n",
    "        x_new = np.float(1)/(np.float(1)+np.float(1)/m)**m\n",
    "        x_dif = x_new - math.exp(-1)\n",
    "        x_lim1 = np.log(np.abs(x_dif))\n",
    "        line1_params = np.polyfit(np.log(1./m), x_lim1, 1)\n",
    "        return line1_params\n",
    "    elif type == 3:\n",
    "        x_new = ((np.float(2)-np.float(1)/m)/(np.float(2)+np.float(1)/m))**m\n",
    "        x_dif = x_new - math.exp(-1)\n",
    "        x_lim1 = np.log(np.abs(x_dif))\n",
    "        line1_params = np.polyfit(np.log(1./m), x_lim1, 1)\n",
    "        return line1_params\n",
    "m = np.array([10, 10**2, 10**3, 10**4, 10**5, 10**6])\n",
    "m.astype(float)\n",
    "x_1 = fproj(m,1)\n",
    "x_2 = fproj(m,2)\n",
    "x_3 = fproj(m,3)\n",
    "print ('The convergence  rate of forward difference Euler method is:'), x_1[0]\n",
    "print ('The convergence  rate of backward difference Euler method is:'), x_2[0]\n",
    "print ('The convergence  rate of central difference Euler method is:'), x_3[0]\n",
    "\n"
   ]
  },
  {
   "cell_type": "markdown",
   "metadata": {},
   "source": [
    "## Implement the schemes discussed above for $f(v) = -v$. Check the correctness of your implementation by using your code to generate approximations  of the Cauchy problem.\n",
    "## The script below implements all of the methods, and then checks the difference between the iterative method's result and exp^(-1)."
   ]
  },
  {
   "cell_type": "code",
   "execution_count": 32,
   "metadata": {
    "collapsed": false
   },
   "outputs": [
    {
     "name": "stdout",
     "output_type": "stream",
     "text": [
      "The time step size is: 1e-05\n",
      "Therefore we iterate the iterative methods until: 100000\n",
      "The returned values from each respective method are: 0.367881280581 0.367881280559 0.367879441167\n",
      "The respective differences for each method are: 1.83940961163e-06 1.83938746495e-06 4.30211422042e-12\n"
     ]
    }
   ],
   "source": [
    "import numpy as np\n",
    "import math\n",
    "def fproj(dt,type,v_new,stop):\n",
    "    m=1\n",
    "    if type ==1:\n",
    "        for i in range(1,stop):\n",
    "            v_new *= (1-dt)\n",
    "            m = m+1\n",
    "        return v_new\n",
    "    elif type ==2:\n",
    "       for i in range(0,stop,1):\n",
    "            v_new *= 1/(1+np.float(dt))\n",
    "       return v_new\n",
    "    elif type == 3:\n",
    "        for i in range(0,stop,1):\n",
    "            v_new *= (2.-dt)/(2.+dt)\n",
    "        return v_new\n",
    "m = 10**5\n",
    "dt = np.float(1)/(m)\n",
    "v_new = float(1)\n",
    "type = 2\n",
    "x_1 = fproj(dt, 1, v_new,m)\n",
    "e_1 = np.abs(x_1 - math.exp(-1))\n",
    "x_2 = fproj(dt, 2, v_new,m)\n",
    "e_2 = np.abs(x_2 - math.exp(-1))\n",
    "x_3 = fproj(dt, 3, v_new,m)\n",
    "e_3 = np.abs(x_3 - math.exp(-1))\n",
    "print ('The time step size is:'), dt \n",
    "print 'Therefore we iterate the iterative methods until:', m\n",
    "print ('The returned values from each respective method are:'), x_1, x_2, x_3\n",
    "print ('The respective differences for each method are:'), e_1, e_2, e_3"
   ]
  },
  {
   "cell_type": "markdown",
   "metadata": {},
   "source": [
    "## (j) Generalize your code to the problem\n",
    "$$ \n",
    "u'(t) = -u^2(t),\\\\\n",
    "u(0) = 1.\n",
    "$$\n",
    "\n",
    "## This requires implementing a different scheme for the backward Euler and central difference Euler. The backward Euler method can be implemented as follows:\n",
    "\n",
    "$$\n",
    "v_{m+1} + \\Delta t v_{m+1}^2 = v_{m}\\\\\n",
    "v_{m+1}^2 + Mv_{m+1} -Mv_{m} = 0,\\qquad \\Delta t = \\frac{1}{M}\\\\\n",
    "v_{m+1} = \\frac{-M \\pm \\sqrt{M^2 + 4Mv_{m}}}{2},\n",
    "$$\n",
    "## which is the final iterative form.\n",
    "## The central difference Euler can be implemented as follows\n",
    "$$\n",
    "v_{m+1} + \\frac{1}{2}\\Delta tv_{m+1}^2 = v_{m}  - \\frac{1}{2}\\Delta tv_{m}^2\\\\\n",
    "v_{m+1} + \\frac{1}{2}\\Delta tv_{m+1}^2 - v_{m} +\\frac{1}{2}\\Delta tv_{m}^2\\\\\n",
    "v_{m+1}^2 + 2Mv_{m+1} + (v_{m}^2 -2Mv_{m})=0\\\\\n",
    "v_{m+1} = -M \\pm \\frac{\\sqrt{(2M)^2 -4(v_{m}^2 -2Mv_{m})}}{2}\\\\\n",
    "V_{M+1} = -M \\pm \\sqrt{(M)^2 -v_{m}^2 +2Mv_{m}}\n",
    "$$\n",
    "## which is the final iterative form."
   ]
  },
  {
   "cell_type": "code",
   "execution_count": 91,
   "metadata": {
    "collapsed": false
   },
   "outputs": [
    {
     "name": "stdout",
     "output_type": "stream",
     "text": [
      "The time step size is: 0.001\n",
      "Therefore we iterate the iterative methods until: 1000 and 10000\n",
      "The returned values from each respective method for number of steps =  1000 are: 0.499826624057 0.500173197769 0.4999999375\n",
      "The returned values from each respective method  for number of steps =  10000 are: 0.090889272353 0.500017327779 0.499999999342\n",
      "The respective differences for each method  for number of steps =  1000 are: 0.000173375943122 0.0001731977693 6.24997937848e-08\n",
      "The respective differences for each method  for number of steps =  10000 are: 0.409092890835 1.73277794602e-05 6.58474164084e-10\n",
      "The rate of convergence of the error of the backward  Euler method is 0.999799382402\n",
      "The rate of convergence of the error of the central Euler method is 1.97733984477\n"
     ]
    }
   ],
   "source": [
    "import numpy as np\n",
    "import math\n",
    "def fproj(dt,type,v_new,stop):\n",
    "    m=1\n",
    "    if type ==1: #Forward Euler method. Needs no modification\n",
    "        for i in range(0,stop,1):\n",
    "            v_old = v_new\n",
    "            v_new = -v_old**2*dt + v_old\n",
    "        return v_new\n",
    "    elif type ==2: #Backwards Euler Method, which requires us to setup an implicit solution using the quadratic equation\n",
    "        for i in range(0,stop,1):\n",
    "            v_old = v_new\n",
    "            v_new = -np.float(stop)/2 + ((np.float(stop)**2 + 4*v_old*stop)**.5)/2\n",
    "        return v_new\n",
    "    elif type == 3:\n",
    "        for i in range(0,stop,1):\n",
    "            v_old = v_new\n",
    "            v_new = -np.float(stop) + 0.5*((2*np.float(stop))**2 - 4*(v_old**2 - 2*np.float(stop)*v_old))**0.5\n",
    "        return v_new\n",
    "\n",
    "m = 10**3\n",
    "m2 = 10**4\n",
    "dt = np.float(1)/(m)\n",
    "v_new = float(1)\n",
    "type = 2\n",
    "y_1 = fproj(dt, 1, v_new,m2)\n",
    "x_1 = fproj(dt, 1, v_new,m)\n",
    "e_1 = np.abs(x_1 - 0.5)\n",
    "E_1 = np.abs(X_1 - 0.5)\n",
    "x_2 = fproj(dt, 2, v_new,m)\n",
    "X_2 = fproj(dt, 2, v_new,m2)\n",
    "E_2 = np.abs(X_2 - 0.5)\n",
    "e_2 = np.abs(x_2 -0.5)\n",
    "x_3 = fproj(dt, 3, v_new,m)\n",
    "X_3 = fproj(dt, 3, v_new,m2)\n",
    "E_3 = np.abs(X_3 - 0.5)\n",
    "e_3 = np.abs(x_3 - 0.5)\n",
    "print ('The time step size is:'), dt \n",
    "print 'Therefore we iterate the iterative methods until:', m, ('and'), m2\n",
    "print ('The returned values from each respective method for number of steps = ') ,m, ('are:'), x_1, x_2, x_3\n",
    "print ('The returned values from each respective method  for number of steps = ') ,m2, ('are:'), y_1, X_2, X_3\n",
    "print ('The respective differences for each method  for number of steps = ') ,m, ('are:'), e_1, e_2, e_3\n",
    "print ('The respective differences for each method  for number of steps = ') ,m2, ('are:'), E_1, E_2, E_3\n",
    "print ('The rate of convergence of the error of the backward  Euler method is'), np.log(e_2/E_2)/(np.log(m2/m))\n",
    "print ('The rate of convergence of the error of the central Euler method is'), np.log(e_3/E_3)/(np.log(m2/m))"
   ]
  },
  {
   "cell_type": "markdown",
   "metadata": {},
   "source": [
    "## (i) Derive the exact solution to this Cauchy problem, and use this to study the error of the three schemes at t = 1.(ii) Do the conclusions of (h) above also apply to the nonlinear problem?\n",
    "## (i)\n",
    "$$\n",
    "u'(t) = \\frac{du}{dt}\\\\\n",
    "\\frac{du}{dt} = -u^2(t)\\\\\n",
    "\\frac{du}{u^2(t)} = -dt\\\\\n",
    "\\int \\frac{du}{u^2(t)} = -t+c\\\\\n",
    "\\frac{1}{u(t)} = t+c\\\\\n",
    "u(t)= \\frac{1}{t+c}\n",
    "$$ \n",
    "## Applying initial conditions\n",
    "$$\n",
    "u(0) = 1 = \\frac{1}{c}\\\\\n",
    "c=1\\\\\n",
    "u(t) = \\frac{1}{1+t}\n",
    "$$\n"
   ]
  },
  {
   "cell_type": "markdown",
   "metadata": {},
   "source": [
    "## The error analysis is carried out above in the script implementing the iterative methods. The central difference method does appear to converge quadratically relative to the forward and backward method, as the error from the central difference method is approximately the square of the error from the forward and backward difference method. However, when using the formula for rate of convergence for the central Euler method, the rate of convergence varies  depending on how many steps are taken. Also, the script bugged consistently when calculating the rate of convergence for the forward Euler method, but is observed that the error is almost equivalent to the error for the backward Euler method."
   ]
  },
  {
   "cell_type": "code",
   "execution_count": null,
   "metadata": {
    "collapsed": true
   },
   "outputs": [],
   "source": []
  }
 ],
 "metadata": {
  "kernelspec": {
   "display_name": "Python [conda root]",
   "language": "python",
   "name": "conda-root-py"
  },
  "language_info": {
   "codemirror_mode": {
    "name": "ipython",
    "version": 2
   },
   "file_extension": ".py",
   "mimetype": "text/x-python",
   "name": "python",
   "nbconvert_exporter": "python",
   "pygments_lexer": "ipython2",
   "version": "2.7.12"
  }
 },
 "nbformat": 4,
 "nbformat_minor": 1
}
